src/refinement/PromisingPF_Promising.v
@@ -21,13 +21,83 @@ Require Import Promising.
 Set Implicit Arguments.
 
 
+(* TODO: move to AlgorithmicPF_Algorithmic. *)
+
+Lemma state_exec_rtc_state_step
+      m1 m2
+      (STEP: Machine.state_exec m1 m2):
+  exists m2',
+    <<EXEC: rtc (Machine.step ExecUnit.state_step) m1 m2'>> /\
+    <<EQUIV: Machine.equiv m2 m2'>>.
+Proof.
+  inv STEP.
+  assert (IN: forall tid sl1
+                (FIND1: IdMap.find tid m1.(Machine.tpool) = Some sl1),
+             exists sl2,
+               IdMap.find tid m2.(Machine.tpool) = Some sl2 /\
+               rtc (ExecUnit.state_step tid)
+                   (ExecUnit.mk sl1.(fst) sl1.(snd) m1.(Machine.mem))
+                   (ExecUnit.mk sl2.(fst) sl2.(snd) m1.(Machine.mem))).
+  { i. specialize (TPOOL tid). rewrite FIND1 in TPOOL. inv TPOOL. esplits; ss. }
+  assert (OUT: forall tid
+                 (FIND1: IdMap.find tid m1.(Machine.tpool) = None),
+             IdMap.find tid m1.(Machine.tpool) = IdMap.find tid m2.(Machine.tpool)).
+  { i. specialize (TPOOL tid). rewrite FIND1 in TPOOL. inv TPOOL. ss. }
+  assert (P: forall tid sl1
+               (FIND1: IdMap.find tid m1.(Machine.tpool) = Some sl1),
+             IdMap.find tid m1.(Machine.tpool) = Some sl1).
+  { ss. }
+  clear TPOOL.
+  setoid_rewrite IdMap.elements_spec in IN at 1.
+  setoid_rewrite IdMap.elements_spec in OUT at 1.
+  setoid_rewrite IdMap.elements_spec in P at 1.
+  generalize (IdMap.elements_3w m1.(Machine.tpool)). intro NODUP. revert NODUP.
+  revert IN OUT P. generalize (IdMap.elements (m1.(Machine.tpool))). intro ps.
+  revert m1 MEM. induction ps; ss.
+  { i. esplits; eauto. econs; ss. ii. rewrite OUT; ss. }
+
+  i. destruct a. inv NODUP.
+  exploit (IN k).
+  { destruct (equiv_dec k k); ss. congr. }
+  exploit (P k).
+  { destruct (equiv_dec k k); ss. congr. }
+  i. des. destruct p. ss.
+
+  cut (exists m2', rtc (Machine.step ExecUnit.state_step)
+                 (Machine.mk (IdMap.add k (sl2.(fst), sl2.(snd)) m1.(Machine.tpool)) m1.(Machine.mem))
+                 m2' /\
+             Machine.equiv m2 m2').
+  { i. des. esplits; [|by eauto]. etrans; [|by eauto].
+    eapply Machine.rtc_eu_step_step; [eauto|refl|eauto].
+  }
+  assert (TID: forall tid sl (FIND: SetoidList.findA (fun id' : IdMap.key => if equiv_dec tid id' then true else false) ps = Some sl), tid <> k).
+  { ii. subst. apply H1. revert FIND. clear. induction ps; ss.
+    destruct a. destruct (equiv_dec k k0); ss.
+    - inv e. i. inv FIND. left. ss.
+    - i. right. apply IHps. ss.
+  }
+  eapply IHps; ss.
+  - i. eapply IN. destruct (equiv_dec tid k); ss.
+    inv e. exfalso. eapply TID; eauto.
+  - i. rewrite IdMap.add_spec. condtac.
+    + inversion e. subst. rewrite x1. destruct sl2. ss.
+    + eapply OUT. destruct (equiv_dec tid k); ss.
+  - i. rewrite IdMap.add_spec. condtac.
+    + inversion e. subst. exfalso. eapply TID; eauto.
+    + eapply P. destruct (equiv_dec tid k); ss.
+Qed.
+
 Theorem promising_pf_to_promising
         p m
         (EXEC: Machine.pf_exec p m):
-  Machine.exec p m.
+  exists m',
+    <<EQUIV: Machine.equiv m m'>> /\
+    <<EXEC: Machine.exec p m'>>.
 Proof.
-  inv EXEC. econs; eauto.
-  etrans.
-  - eapply Machine.rtc_step_mon; cycle 1; eauto. right. ss.
-  - eapply Machine.rtc_step_mon; cycle 1; eauto. left. ss.
+  inv EXEC. exploit state_exec_rtc_state_step; eauto. i. des.
+  esplits; eauto. econs.
+  - etrans.
+    + eapply rtc_mon; [|by eauto]. apply Machine.step_mon. right. ss.
+    + eapply rtc_mon; [|by eauto]. apply Machine.step_mon. left. ss.
+  - eapply Machine.equiv_no_promise; eauto.
 Qed.
